fairness/fuel.v
@@ -43,6 +43,23 @@ Section fairness.
   Global Instance FL_eqdec: EqDecision (@FairLabel (fmrole M)).
   Proof. solve_decision. Qed.
 
+  Global Instance FL_cnt: Countable (@FairLabel (fmrole M)).
+  Proof. 
+    set (FL_alt := (G * (fmrole M) + G + unit)%type).
+    set (to_alt := fun fl => match fl with
+                          | Take_step ρ τ => inl $ inl (τ, ρ)
+                          | Silent_step τ => inl $ inr τ
+                          | Config_step => (inr tt): FL_alt
+                          end).
+    set (from_alt := fun (fl': FL_alt) => match fl' with
+                             | inl (inl (τ, ρ)) => Take_step ρ τ
+                             | inl (inr τ) => Silent_step τ
+                             | inr _ => Config_step
+                             end).
+    eapply (inj_countable' to_alt from_alt).
+    intros. by destruct x. 
+  Qed. 
+
   Definition less (x y: option nat) :=
     match x, y with
     | Some x, Some y => x < y
@@ -59,6 +76,20 @@ Section fairness.
   (* | Zombie otid (Hismainrole: oρ = Some ρ') (Hnotalive: ρ' ∉ live_roles _ b) (Hnotdead: ρ' ∈ dom b.(ls_fuel)): *)
   (*   must_decrease ρ' oρ a b otid *)
   .
+
+  Global Instance must_decrease_dec:
+    forall a oρ st1 st2 og, Decision (must_decrease a oρ st1 st2 og).
+  Proof. 
+    intros.
+    destruct (decide (@ls_mapping st1 !! a ≠ @ls_mapping st2 !! a /\ is_Some (@ls_mapping st2 !! a))).
+    { left. apply Change_tid; apply a0. }
+    destruct og.
+    2: { right. intros DECR. inversion DECR; tauto. }
+    destruct (decide (Some a ≠ oρ /\ Some g = @ls_mapping st1 !! a)).
+    - left. econstructor; apply a0.
+    - right. intros DECR. inversion DECR; tauto.
+  Qed.
+
 
   Definition fuel_decr (tid: option G) (oρ: option M.(fmrole))
              (a b: LiveState) :=
@@ -106,6 +137,18 @@ Section fairness.
       lm_ls_trans := ls_trans lm_fl;
     }.
   
+  Definition fair_lbl_matches_group (ℓ: @FairLabel (fmrole M)) (τ: G) := 
+    match ℓ with
+    | Take_step _ τ' | Silent_step τ' => τ = τ'
+    | Config_step => False
+    end. 
+
+  Global Instance fair_lbl_match_Dec: 
+    forall ℓ τ, Decision (fair_lbl_matches_group ℓ τ).
+  Proof.
+    intros. destruct ℓ; simpl; solve_decision.
+  Qed.  
+
   Definition live_model_model `(LM : LiveModel) : Model := {|
     mstate := lm_ls LM;
     mlabel := lm_lbl LM;
@@ -137,6 +180,80 @@ Section fairness.
     done.
   Qed. 
 
+  Local Ltac SS' := eapply elem_of_dom; eauto. 
+
+  Lemma others_step_fuel_decr `{LM: LiveModel} ρ f f' τ δ ℓ δ'
+    (STEP: lm_ls_trans LM δ ℓ δ')
+    (Hfuel : @ls_fuel δ !! ρ = Some f)
+    (Hmapping : @ls_mapping δ !! ρ = Some τ)
+    (Hζ: ¬ fair_lbl_matches_group ℓ τ)
+    (FUEL: @ls_fuel δ' !! ρ = Some f'):
+    f' ≤ f.
+  Proof.
+    simpl in *. destruct ℓ as [ρ0 ζ0| ζ0|]; try done.
+    + destruct STEP as (?&?&?&Hnoninc&?).
+      unfold fuel_must_not_incr in Hnoninc.
+      have Hneq: Some ρ ≠ Some ρ0 by congruence.
+      specialize (Hnoninc ρ ltac:(SS')).
+      unfold oleq in Hnoninc. rewrite Hfuel in Hnoninc.
+      rewrite FUEL in Hnoninc.
+      destruct Hnoninc as [?|[?|C]]. 
+      3: { destruct (proj1 C). eapply elem_of_dom; eauto. }
+      all: set_solver. 
+    + destruct STEP as (?&?&Hnoninc&?).
+      unfold fuel_must_not_incr in Hnoninc.
+      have Hneq: Some ρ ≠ None by congruence.
+      specialize (Hnoninc ρ ltac:(SS')).
+      unfold oleq in Hnoninc. rewrite Hfuel in Hnoninc.
+      rewrite FUEL in Hnoninc. 
+      destruct Hnoninc as [?|[?|C]]. 
+      3: { destruct (proj1 C). eapply elem_of_dom; eauto. }
+      all: set_solver.
+    + destruct STEP as [_ [_ [Hnoninc _]]].
+      have HnotNone: Some ρ ≠ None by congruence.
+      specialize (Hnoninc ρ ltac:(SS')).
+      unfold oleq in Hnoninc. rewrite Hfuel in Hnoninc.
+      rewrite FUEL in Hnoninc. 
+      destruct Hnoninc as [?|[?|C]]. 
+      3: { destruct (proj1 C). eapply elem_of_dom; eauto. }
+      all: set_solver.
+  Qed. 
+  
+  Lemma owner_change_fuel_decr `{LM: LiveModel} ρ f f'
+    δ ℓ δ'
+    τ τ''
+    (STEP: lm_ls_trans LM δ ℓ δ')
+    (Hfuel: @ls_fuel δ !! ρ = Some f)
+    (Hmapping: @ls_mapping δ !! ρ = Some τ)
+    (Hζ'' : @ls_mapping δ' !! ρ = Some τ'')
+    (Hchange : τ ≠ τ'')
+    (FUEL: @ls_fuel δ' !! ρ = Some f'):
+    f' < f.
+  Proof.
+    destruct ℓ as [ρ0 ζ0| ζ0|]; try done.
+    + destruct STEP as (?&?&Hdec&?&?).
+      unfold fuel_decr in Hdec. simplify_eq.
+      have Hmd: must_decrease ρ (Some ρ0) δ δ' (Some ζ0).
+      { econstructor 2. congruence. rewrite Hζ''; eauto. }
+      specialize (Hdec ρ ltac:(SS') ltac:(SS') Hmd).
+      unfold oleq in Hdec. rewrite Hfuel in Hdec.
+      by rewrite FUEL in Hdec. 
+    + destruct STEP as (?&Hdec&_).
+      unfold fuel_decr in Hdec. simplify_eq.
+      have Hmd: must_decrease ρ None δ δ' (Some ζ0).
+      { econstructor 2. congruence. rewrite Hζ''; eauto. }
+      specialize (Hdec ρ ltac:(SS') ltac:(SS') Hmd).
+      unfold oleq in Hdec. rewrite Hfuel in Hdec.
+      by rewrite FUEL in Hdec.
+    + destruct STEP as [_ [Hdec _]].
+      unfold fuel_decr in Hdec.
+      have Hmd: must_decrease ρ None δ δ' None.
+      { econstructor. congruence. rewrite Hζ''. eauto. }
+      specialize (Hdec ρ ltac:(SS') ltac:(SS') Hmd).
+      unfold oleq in Hdec. rewrite Hfuel in Hdec.
+      by rewrite FUEL in Hdec.
+  Qed.
+
 End fairness.
 
 Arguments LiveState : clear implicits.
@@ -149,805 +266,3 @@ Coercion live_model_to_model : LiveModel >-> Model.
 Arguments live_model_to_model {_ _}.
 
 
-Section aux_trace.  
-  Context `{LM: LiveModel G M LSI}.
-  Context `{Countable G}.
-
-  Definition auxtrace := trace LM.(lm_ls) LM.(lm_lbl).
-
-  Definition role_enabled ρ (δ: LiveState G M LSI) := ρ ∈ M.(live_roles) δ.
-
-  Definition lbl_with_role (ρ: fmrole M) (ℓ: lm_lbl LM) := 
-    ∃ tid, ℓ = Take_step ρ tid. 
-
-  (* Definition fair_aux ρ (auxtr: auxtrace ): Prop  := *)
-  (*   forall n, pred_at auxtr n (λ δ _, role_enabled ρ δ) -> *)
-  (*        ∃ m, pred_at auxtr (n+m) (λ δ _, ¬role_enabled ρ δ) *)
-  (*             ∨ pred_at auxtr (n+m) (λ _ ℓ, ∃ tid, ℓ = Some (Take_step ρ tid)). *)
-  Definition fair_aux := fair_by role_enabled lbl_with_role. 
-  
-  (* Lemma fair_aux_after ρ auxtr n auxtr': *)
-  (*   fair_aux ρ auxtr -> *)
-  (*   after n auxtr = Some auxtr' -> *)
-  (*   fair_aux ρ auxtr'. *)
-  (* Proof. *)
-  (*   rewrite /fair_aux => Hfair Hafter m Hpa. *)
-  (*   specialize (Hfair (n+m)). *)
-  (*   rewrite -> (pred_at_sum _ n) in Hfair. rewrite Hafter in Hfair. *)
-  (*   destruct (Hfair Hpa) as (p&Hp). *)
-  (*   exists (p). by rewrite <-Nat.add_assoc, ->!(pred_at_sum _ n), Hafter in Hp. *)
-  (* Qed. *)
-
-  CoInductive auxtrace_valid: auxtrace -> Prop :=
-  | auxtrace_valid_singleton δ: auxtrace_valid ⟨δ⟩
-  | auxtrace_valid_cons δ ℓ tr:
-      LM.(lm_ls_trans) δ ℓ (trfirst tr) ->
-      auxtrace_valid tr →
-      auxtrace_valid (δ -[ℓ]-> tr).
-
-  Lemma auxtrace_valid_forall (tr: auxtrace) :
-    auxtrace_valid tr ->
-    ∀ n, match after n tr with
-         | Some ⟨ _ ⟩ | None => True
-         | Some (δ -[ℓ]-> tr') => LM.(lm_ls_trans) δ ℓ (trfirst tr')
-         end.
-  Proof.
-    intros Hval n. revert tr Hval. induction n as [|n]; intros tr Hval;
-      destruct (after _ tr) as [trn|] eqn: Heq =>//; simpl in Heq;
-      simplify_eq; destruct trn =>//; inversion Hval; simplify_eq; try done.
-    specialize (IHn _ H1) (* TODO *). rewrite Heq in IHn. done.
-  Qed.
-
-  Lemma auxtrace_valid_after (tr: auxtrace):
-    auxtrace_valid tr ->
-    forall n atr, after n tr = Some atr -> auxtrace_valid atr.
-  Proof. 
-    intros VALID n. generalize dependent tr. induction n.
-    { intros. rewrite after_0_id in H0. congruence. }  
-    intros. inversion VALID; subst. 
-    { done. }
-    simpl in H0. eauto.
-  Qed. 
-    
-End aux_trace.
-
-Section aux_trace_lang.
-  Context `{LM: LiveModel (locale Λ) M LSI}.
-  Context `{Countable (locale Λ)}.
-
-  Notation "'Tid'" := (locale Λ). 
-
-  Definition tids_smaller (c : list (expr Λ)) (δ: LiveState Tid M LSI) :=
-    ∀ ρ ζ, δ.(ls_mapping) !! ρ = Some ζ -> is_Some (from_locale c ζ).
-
-  Definition labels_match (oζ : option Tid) (ℓ : LM.(lm_lbl)) : Prop :=
-    match oζ, ℓ with
-    | None, Config_step => True
-    | Some ζ, Silent_step ζ' => ζ = ζ'
-    | Some ζ, Take_step ρ ζ' => ζ = ζ'
-    | _, _ => False
-    end.
-
-End aux_trace_lang.
-
-Ltac SS :=
-  epose proof ls_fuel_dom;
-  (* epose proof ls_mapping_dom; *)
-  set_solver.
-
-Definition live_tids `{LM:LiveModel (locale Λ) M LSI} `{EqDecision (locale Λ)}
-           (c : cfg Λ) (δ : LM.(lm_ls)) : Prop :=
-  (∀ ρ ζ, δ.(ls_mapping (G := locale Λ)) !! ρ = Some ζ -> is_Some (from_locale c.1 ζ)) ∧
-  ∀ ζ e, from_locale c.1 ζ = Some e -> (to_val e ≠ None) ->
-         ∀ ρ, δ.(ls_mapping) !! ρ ≠ Some ζ.
-
-(* TODO: replace original definition with this *)
-Lemma live_tids_alt `{LM:LiveModel (locale Λ) M LSI} `{EqDecision (locale Λ)} c δ:
-  live_tids c δ (LM := LM) (Λ := Λ) <->
-    (forall ζ, (exists ρ, ls_mapping δ !! ρ = Some ζ) ->
-          locale_enabled ζ c).
-Proof.
-  rewrite /live_tids /locale_enabled. split.
-  - intros. destruct H0 as [ρ MAP].
-    destruct H as [EXPR NVAL].
-    specialize (EXPR _ _ MAP) as [e ?].
-    eexists. split; eauto.
-    specialize (NVAL _ _ H). 
-    destruct (to_val e); [| done].
-    specialize (NVAL ltac:(eauto)).
-    edestruct NVAL; eauto.
-  - intros. split.
-    + intros. specialize (H ζ (@ex_intro _ _ _ H0)) as [e [MAP ?]].
-      eauto.
-    + intros. intros MAP.
-      specialize (H ζ (@ex_intro _ _ _ MAP)) as [? [? NVAL]].
-      congruence.
-Qed.
-
-(* Definition exaux_traces_match `{LM:LiveModel (locale Λ) M} `{EqDecision (locale Λ)} : *)
-(*   extrace Λ → auxtrace (LM := LM) → Prop := *)
-(*   traces_match labels_match *)
-(*                live_tids *)
-(*                locale_step *)
-(*                LM.(lm_ls_trans). *)
-
-
-Definition valid_evolution_step `{LM:LiveModel (locale Λ) M LSI} `{EqDecision (locale Λ)}
-  oζ (σ2: cfg Λ) δ1 ℓ δ2 :=
-    labels_match (LM:=LM) oζ ℓ ∧ LM.(lm_ls_trans) δ1 ℓ δ2 ∧
-    tids_smaller (σ2.1) δ2.
-
-(* TODO: get rid of previous version *)
-Definition lm_valid_evolution_step `{LM:LiveModel (locale Λ) M LSI} `{EqDecision (locale Λ)}:
-    cfg Λ → olocale Λ → cfg Λ → 
-    mstate LM → lm_lbl LM → mstate LM -> Prop := 
-    (fun (_: cfg Λ) => valid_evolution_step).
-
-(* Section fairness_preserved. *)
-(*   Context `{LM: LiveModel (locale Λ) M}. *)
-(*   Context `{Countable (locale Λ)}. *)
-(*   Notation "'Tid'" := (locale Λ).  *)
-
-(*   Lemma exaux_preserves_validity extr (auxtr : auxtrace (LM := LM)): *)
-(*     exaux_traces_match extr auxtr -> *)
-(*     auxtrace_valid auxtr. *)
-(*   Proof. *)
-(*     revert extr auxtr. cofix CH. intros extr auxtr Hmatch. *)
-(*     inversion Hmatch; first by constructor. *)
-(*     constructor =>//. by eapply CH. *)
-(*   Qed. *)
-
-(*   Lemma exaux_preserves_termination extr (auxtr : auxtrace (LM := LM)) : *)
-(*     exaux_traces_match extr auxtr -> *)
-(*     terminating_trace auxtr -> *)
-(*     terminating_trace extr. *)
-(*   Proof. *)
-(*     intros Hmatch [n HNone]. *)
-(*     revert extr auxtr Hmatch HNone. induction n as [|n IHn]; first done. *)
-(*     intros extr auxtr Hmatch HNone. *)
-(*     replace (S n) with (1 + n) in HNone =>//. *)
-(*     rewrite (after_sum' _ 1) in HNone. *)
-(*     destruct auxtr as [s| s ℓ auxtr']; *)
-(*       first by inversion Hmatch; simplify_eq; exists 1. *)
-(*     simpl in HNone. *)
-(*     inversion Hmatch; simplify_eq. *)
-(*     apply terminating_trace_cons. *)
-(*     eapply IHn =>//. *)
-(*   Qed. *)
-
-(*   Lemma traces_match_labels tid ℓ c δ rex (raux : auxtrace (LM := LM)) : *)
-(*     exaux_traces_match (c -[Some tid]-> rex) (δ -[ℓ]-> raux) -> *)
-(*     ((∃ ρ, ℓ = Take_step ρ tid) ∨ (ℓ = Silent_step tid)). *)
-(*   Proof. *)
-(*     intros Hm. inversion Hm as [|?????? Hlab]; simplify_eq. *)
-(*     destruct ℓ; eauto; inversion Hlab; simplify_eq; eauto. *)
-(*   Qed. *)
-
-(*   Lemma mapping_live_role (δ: LiveState Tid M) ρ: *)
-(*     ρ ∈ M.(live_roles) δ -> *)
-(*     is_Some (ls_mapping (G := Tid) δ !! ρ). *)
-(*   Proof. rewrite -elem_of_dom ls_same_doms. SS. Qed. *)
-(*   Lemma fuel_live_role (δ: LiveState Tid M) ρ: *)
-(*     ρ ∈ M.(live_roles) δ -> *)
-(*     is_Some (ls_fuel (G := Tid) δ !! ρ). *)
-(*   Proof. rewrite -elem_of_dom. SS. Qed. *)
-
-(*   Local Hint Resolve mapping_live_role: core. *)
-(*   Local Hint Resolve fuel_live_role: core. *)
-
-(*   Lemma match_locale_enabled (extr : extrace Λ) (auxtr : auxtrace (LM := LM)) ζ ρ: *)
-(*     exaux_traces_match extr auxtr -> *)
-(*     ls_mapping (trfirst auxtr) !! ρ = Some ζ -> *)
-(*     locale_enabled ζ (trfirst extr). *)
-(*   Proof. *)
-(*     intros Hm Hloc. *)
-(*     rewrite /locale_enabled. have [HiS Hneqloc] := traces_match_first _ _ _ _ _ _ Hm. *)
-(*     have [e Hein] := (HiS _ _ Hloc). exists e. split; first done. *)
-(*     destruct (to_val e) eqn:Heqe =>//. *)
-(*     exfalso. specialize (Hneqloc ζ e Hein). rewrite Heqe in Hneqloc. *)
-(*     have Hv: Some v ≠ None by []. by specialize (Hneqloc Hv ρ). *)
-(*   Qed. *)
-
-(*   Local Hint Resolve match_locale_enabled: core. *)
-(*   Local Hint Resolve pred_first_trace: core. *)
-
-(*   Definition fairness_induction_stmt ρ fm f m ζ extr (auxtr : auxtrace (LM := LM)) *)
-(*     δ c := *)
-(*       (infinite_trace extr -> *)
-(*        (forall ζ, fair_ex ζ extr) -> *)
-(*        fm = (f, m) -> *)
-(*        exaux_traces_match extr auxtr -> *)
-(*        c = trfirst extr -> δ = trfirst auxtr -> *)
-(*        δ.(ls_fuel) !! ρ = Some f -> *)
-(*        δ.(ls_mapping) !! ρ = Some ζ -> *)
-(*        (pred_at extr m (λ c _, ¬locale_enabled ζ c) ∨ pred_at extr m (λ _ oζ, oζ = Some (Some ζ))) -> *)
-(*       ∃ M, pred_at auxtr M (λ δ _, ¬role_enabled ρ δ) *)
-(*            ∨ pred_at auxtr M (λ _ ℓ, ∃ ζ0, ℓ = Some (Take_step ρ ζ0))). *)
-
-(*   Local Lemma case1 ρ f m (extr' : extrace Λ) (auxtr' : auxtrace (LM := LM)) δ ℓ : *)
-(*     (∀ m0 : nat * nat, *)
-(*          strict lt_lex m0 (f, m) *)
-(*          → ∀ (f m: nat) (ζ: locale Λ) (extr : extrace Λ) (auxtr : auxtrace (LM := LM)) *)
-(*              (δ : LiveState Tid M) (c : cfg Λ), fairness_induction_stmt ρ m0 f m ζ extr auxtr δ c) -> *)
-(*     (ρ ∈ dom (ls_fuel (trfirst auxtr')) → oless (ls_fuel (trfirst auxtr') !! ρ) (ls_fuel δ !! ρ)) -> *)
-(*     exaux_traces_match extr' auxtr' -> *)
-(*     infinite_trace extr' -> *)
-(*     ls_fuel δ !! ρ = Some f -> *)
-(*     (∀ ζ, fair_ex ζ extr') -> *)
-(*     ∃ M0 : nat, *)
-(*       pred_at (δ -[ ℓ ]-> auxtr') M0 *)
-(*               (λ δ0 _, ¬ role_enabled ρ δ0) *)
-(*       ∨ pred_at (δ -[ ℓ ]-> auxtr') M0 *)
-(*                 (λ _ ℓ, ∃ ζ0, ℓ = Some (Take_step ρ ζ0)). *)
-(*     Proof. *)
-(*       intros IH Hdec Hmatch Hinf Hsome Hfair. *)
-(*       unfold oless in Hdec. *)
-(*       simpl in *. *)
-(*       rewrite -> Hsome in *. *)
-(*       destruct (ls_fuel (trfirst auxtr') !! ρ) as [f'|] eqn:Heq. *)
-(*       - destruct (decide (ρ ∈ live_roles M (trfirst auxtr'))) as [Hρlive'|]; last first. *)
-(*         { exists 1. left. unfold pred_at. simpl. destruct auxtr'; eauto. } *)
-(*         have [ζ' Hζ'] : is_Some (ls_mapping (trfirst auxtr') !! ρ) by eauto. *)
-
-(*         have Hloc'en: pred_at extr' 0 (λ (c : cfg Λ) (_ : option (olocale Λ)), *)
-(*                           locale_enabled ζ' c). *)
-(*         { rewrite /pred_at /= pred_first_trace. eauto. } *)
-
-(*         have [p Hp] := (Hfair ζ' 0 Hloc'en). *)
-(*         have [P Hind] : ∃ M0 : nat, pred_at auxtr' M0 (λ (δ0 : LiveState Tid M) _, ¬ role_enabled ρ δ0) *)
-(*                                   ∨ pred_at auxtr' M0 (λ (_ : LiveState Tid M) ℓ, ∃ ζ0, ℓ = Some (Take_step ρ ζ0)). *)
-(*         { eapply (IH _ _ _ p _ extr'); eauto. *)
-(*           Unshelve. unfold strict, lt_lex. specialize (Hdec ltac:(by eapply elem_of_dom_2)). lia. } *)
-(*         exists (1+P). rewrite !pred_at_sum. simpl. done. *)
-(*       - exists 1. left. rewrite /pred_at /=. rewrite /role_enabled. *)
-(*         destruct auxtr' =>/=. *)
-(*         + apply not_elem_of_dom in Heq; eapply not_elem_of_weaken; last (by apply ls_fuel_dom); set_solver. *)
-(*         + apply not_elem_of_dom in Heq; eapply not_elem_of_weaken; last (by apply ls_fuel_dom); set_solver. *)
-(*     Qed. *)
-
-(*   Lemma fairness_preserved_ind ρ: *)
-(*     ∀ fm f m ζ (extr: extrace Λ) (auxtr: auxtrace (LM := LM)) δ c, *)
-(*       fairness_induction_stmt ρ fm f m ζ extr auxtr δ c. *)
-(*   Proof. *)
-(*     induction fm as [fm IH] using lex_ind. *)
-(*     intros f m ζ extr auxtr δ c Hexinfin Hfair -> Htm -> -> Hfuel Hmapping Hexen. *)
-(*     destruct extr as [|c ζ' extr'] eqn:Heq. *)
-(*     { have [??] := Hexinfin 1. done. } *)
-(*     have Hfair': (forall ζ, fair_ex ζ extr'). *)
-(*     { intros. by eapply fair_ex_cons. } *)
-(*     destruct auxtr as [|δ ℓ auxtr']; first by inversion Htm. *)
-(*     destruct (decide (ρ ∈ live_roles M δ)) as [Hρlive|]; last first. *)
-(*     { exists 0. left. unfold pred_at. simpl. intros contra. eauto. } *)
-(*     destruct (decide (Some ζ = ζ')) as [Hζ|Hζ]. *)
-(*     - rewrite <- Hζ in *. *)
-(*       destruct (traces_match_labels _ _ _ _ _ _ Htm) as [[ρ' ->]| ->]; last first. *)
-(*       + inversion Htm as [|s1 ℓ1 r1 s2 ℓ2 r2 Hl Hs Hts Hls Hmatchrest]; simplify_eq. *)
-(*         unfold ls_trans in Hls. *)
-(*         destruct Hls as (? & Hlsdec & Hlsincr). *)
-(*         unfold fuel_decr in Hlsdec. *)
-(*         have Hmustdec: must_decrease ρ None δ (trfirst auxtr') (Some ζ). *)
-(*         { constructor; eauto. } *)
-(*         eapply case1 =>//. *)
-(*         * move=> Hinfuel; apply Hlsdec => //; first set_solver. *)
-(*         * eapply infinite_cons =>//. *)
-(*       + (* Three cases: *) *)
-(* (*            (1) ρ' = ρ and we are done *) *)
-(* (*            (2) ρ' ≠ ρ but they share the same ρ -> ρ decreases *) *)
-(* (*            (3) ρ' ≠ ρ and they don't have the same tid -> *) *)
-(* (*            impossible because tid and the label must match! *) *)
-(*         inversion Htm as [|s1 ℓ1 r1 s2 ℓ2 r2 Hl Hs Hts Hls Hmatchrest]; simplify_eq. *)
-(*         destruct (decide (ρ = ρ')) as [->|Hρneq]. *)
-(*         { exists 0. right. rewrite /pred_at /=. eauto. } *)
-(*         destruct Hls as (?&Hsame&Hdec&Hnotinc&_). *)
-(*         rewrite -Hsame /= in Hmapping. *)
-(*         have Hmustdec: must_decrease ρ (Some ρ') δ (trfirst auxtr') (Some ζ). *)
-(*         { constructor; eauto; congruence. } *)
-(*         (* Copy and paste begins here *) *)
-(*         eapply case1 =>//; last by eauto using infinite_cons. *)
-(*         intros Hinfuels. apply Hdec =>//. SS. *)
-(*     - (* Another thread is taking a step. *) *)
-(*       destruct (decide (ρ ∈ live_roles M (trfirst auxtr'))) as [Hρlive'|]; last first. *)
-(*       { exists 1. left. unfold pred_at. simpl. destruct auxtr'; eauto. } *)
-(*       have [ζ'' Hζ''] : is_Some (ls_mapping (trfirst auxtr') !! ρ) by eauto. *)
-(*       destruct (decide (ζ = ζ'')) as [<-|Hchange]. *)
-(*       + have [f' [Hfuel' Hff']] : exists f', ls_fuel (trfirst auxtr') !! ρ = Some f' ∧ f' ≤ f. *)
-(*         { destruct ζ' as [ζ'|]; last first; simpl in *. *)
-(*           - inversion Htm as [|s1 ℓ1 r1 s2 ℓ2 r2 Hl Hs Hts Hls Hmatchrest]; simplify_eq. *)
-(*             simpl in *. destruct ℓ; try done. destruct Hls as [_ [_ [Hnoninc _]]]. *)
-(*             have HnotNone: Some ρ ≠ None by congruence. *)
-(*             (* specialize (Hnoninc ρ ltac:(SS) HnotNone). *) *)
-(*             specialize (Hnoninc ρ ltac:(SS)). *)
-(*             unfold oleq in Hnoninc. rewrite Hfuel in Hnoninc. *)
-(*             destruct (ls_fuel (trfirst auxtr') !! ρ) as [f'|] eqn:Heq; [|set_solver]. *)
-(*             eexists; split =>//. destruct Hnoninc as [Hnoninc|Hnoninc]=>//. *)
-(*             apply elem_of_dom_2 in Heq. set_solver. *)
-(*           - inversion Htm as [|s1 ℓ1 r1 s2 ℓ2 r2 Hl Hs Hts Hls Hmatchrest]; simplify_eq. *)
-(*             simpl in *. destruct ℓ as [ρ0 ζ0| ζ0|]; try done. *)
-(*             + destruct Hls as (?&?&?&Hnoninc&?). *)
-(*               unfold fuel_must_not_incr in Hnoninc. *)
-(*               have Hneq: Some ρ ≠ Some ρ0 by congruence. *)
-(*               (* specialize (Hnoninc ρ ltac:(SS) Hneq). *) *)
-(*               specialize (Hnoninc ρ ltac:(SS)). *)
-(*               unfold oleq in Hnoninc. rewrite Hfuel in Hnoninc. *)
-(*               destruct (ls_fuel (trfirst auxtr') !! ρ) as [f'|] eqn:Heq; [|set_solver]. *)
-(*               eexists; split =>//. destruct Hnoninc as [Hnoninc|Hnoninc]=>//. *)
-(*               apply elem_of_dom_2 in Heq. set_solver. *)
-(*             + destruct Hls as (?&?&Hnoninc&?). *)
-(*               unfold fuel_must_not_incr in Hnoninc. *)
-(*               have Hneq: Some ρ ≠ None by congruence. *)
-(*               (* specialize (Hnoninc ρ ltac:(SS) Hneq). *) *)
-(*               specialize (Hnoninc ρ ltac:(SS)). *)
-(*               unfold oleq in Hnoninc. rewrite Hfuel in Hnoninc. *)
-(*               destruct (ls_fuel (trfirst auxtr') !! ρ) as [f'|] eqn:Heq; [|set_solver]. *)
-(*               eexists; split =>//. destruct Hnoninc as [Hnoninc|Hnoninc]=>//. *)
-(*               apply elem_of_dom_2 in Heq. set_solver. } *)
-
-(*         unfold fair_ex in *. *)
-(*         have Hζ'en: pred_at extr' 0 (λ (c : cfg Λ) _, locale_enabled ζ c). *)
-(*         { rewrite /pred_at /= pred_first_trace. inversion Htm; eauto. } *)
-(*         destruct m as [| m']. *)
-(*         { rewrite -> !pred_at_0 in Hexen. destruct Hexen as [Hexen|Hexen]. *)
-(*           - exfalso. apply Hexen. unfold locale_enabled. by eapply (match_locale_enabled _ _ _ _ Htm). *)
-(*           - simplify_eq. } *)
-
-(*         have [P Hind] : ∃ M0 : nat, pred_at auxtr' M0 (λ δ0 _, ¬ role_enabled ρ δ0) *)
-(*                         ∨ pred_at auxtr' M0 (λ _ ℓ, ∃ ζ0, ℓ = Some (Take_step ρ ζ0)). *)
-(*         { eapply (IH _ _ _ m' _ extr'); eauto. by eapply infinite_cons. by inversion Htm. *)
-(*           Unshelve. unfold strict, lt_lex. lia. } *)
-(*         exists (1+P). rewrite !pred_at_sum. simpl. done. *)
-(*       + have [f' [Hfuel' Hff']] : exists f', ls_fuel (trfirst auxtr') !! ρ = Some f' ∧ f' < f. *)
-(*         { destruct ζ' as [ζ'|]; last first; simpl in *. *)
-(*           - inversion Htm as [|s1 ℓ1 r1 s2 ℓ2 r2 Hl Hs Hts Hls Hmatchrest]; simplify_eq. *)
-(*             simpl in *. destruct ℓ; try done. destruct Hls as [_ [Hdec _]]. *)
-(*             unfold fuel_decr in Hdec. *)
-(*             have Hmd: must_decrease ρ None δ (trfirst auxtr') None. *)
-(*             { econstructor. congruence. rewrite Hζ''. eauto. } *)
-(*             specialize (Hdec ρ ltac:(SS) ltac:(SS) Hmd). *)
-(*             unfold oleq in Hdec. rewrite Hfuel in Hdec. *)
-(*             destruct (ls_fuel (trfirst auxtr') !! ρ) as [f'|] eqn:Heq; [by eexists|done]. *)
-(*           - inversion Htm as [|s1 ℓ1 r1 s2 ℓ2 r2 Hl Hs Hts Hls Hmatchrest]; simplify_eq. *)
-(*             simpl in *. destruct ℓ as [ρ0 ζ0| ζ0|]; try done. *)
-(*             + destruct Hls as (?&?&Hdec&?&?). *)
-(*               unfold fuel_decr in Hdec. simplify_eq. *)
-(*               have Hmd: must_decrease ρ (Some ρ0) δ (trfirst auxtr') (Some ζ0). *)
-(*               { econstructor 2. congruence. rewrite Hζ''; eauto. } *)
-(*               specialize (Hdec ρ ltac:(SS) ltac:(SS) Hmd). *)
-(*               unfold oleq in Hdec. rewrite Hfuel in Hdec. *)
-(*               destruct (ls_fuel (trfirst auxtr') !! ρ) as [f'|] eqn:Heq; [by eexists|done]. *)
-(*             + destruct Hls as (?&Hdec&_). *)
-(*               unfold fuel_decr in Hdec. simplify_eq. *)
-(*               have Hmd: must_decrease ρ None δ (trfirst auxtr') (Some ζ0). *)
-(*               { econstructor 2. congruence. rewrite Hζ''; eauto. } *)
-(*               specialize (Hdec ρ ltac:(SS) ltac:(SS) Hmd). *)
-(*               unfold oleq in Hdec. rewrite Hfuel in Hdec. *)
-(*               destruct (ls_fuel (trfirst auxtr') !! ρ) as [f'|] eqn:Heq; [by eexists|done]. } *)
-
-(*         unfold fair_ex in *. *)
-(*         have: pred_at extr' 0 (λ c _, locale_enabled ζ'' c). *)
-(*         { rewrite /pred_at /= pred_first_trace. inversion Htm; eauto. } *)
-(*         have Hζ'en: pred_at extr' 0 (λ c _, locale_enabled ζ'' c). *)
-(*         { rewrite /pred_at /= pred_first_trace. inversion Htm; eauto. } *)
-(*         have [p Hp] := (Hfair' ζ'' 0 Hζ'en). *)
-(*         have [P Hind] : ∃ M0 : nat, pred_at auxtr' M0 (λ δ0 _, ¬ role_enabled ρ δ0) *)
-(*                         ∨ pred_at auxtr' M0 (λ _ ℓ, ∃ ζ0, ℓ = Some (Take_step ρ ζ0)). *)
-(*         { eapply (IH _ _ _ p _ extr'); eauto. by eapply infinite_cons. by inversion Htm. *)
-(*           Unshelve. unfold strict, lt_lex. lia. } *)
-(*         exists (1+P). rewrite !pred_at_sum. simpl. done. *)
-(*   Qed. *)
-
-(*   Theorem fairness_preserved (extr: extrace Λ) (auxtr: auxtrace (LM := LM)): *)
-(*     infinite_trace extr -> *)
-(*     exaux_traces_match extr auxtr -> *)
-(*     (forall ζ, fair_ex ζ extr) -> (forall ρ, fair_aux ρ auxtr). *)
-(*   Proof. *)
-(*     intros Hinfin Hmatch Hex ρ n Hn. *)
-(*     unfold pred_at in Hn. *)
-(*     destruct (after n auxtr) as [tr|] eqn:Heq =>//. *)
-(*     setoid_rewrite pred_at_sum. rewrite Heq. *)
-(*     have Hen: role_enabled ρ (trfirst tr) by destruct tr. *)
-(*     have [ζ Hζ] : is_Some((trfirst tr).(ls_mapping) !! ρ) by eauto. *)
-(*     have [f Hfuel] : is_Some((trfirst tr).(ls_fuel) !! ρ) by eauto. *)
-(*     have Hex' := Hex ζ n. *)
-(*     have [tr1' [Heq' Htr]] : exists tr1', after n extr = Some tr1' ∧ exaux_traces_match tr1' tr *)
-(*      by eapply traces_match_after. *)
-(*     have Hte: locale_enabled ζ (trfirst tr1'). *)
-(*     { rewrite /locale_enabled. have [HiS Hneqζ] := traces_match_first _ _ _ _ _ _ Htr. *)
-(*       have [e Hein] := (HiS _ _ Hζ). exists e. split; first done. *)
-(*       destruct (to_val e) eqn:Heqe =>//. *)
-(*       exfalso. specialize (Hneqζ ζ e Hein). rewrite Heqe in Hneqζ. *)
-(*       have HnotNull: Some v ≠ None by []. specialize (Hneqζ HnotNull ρ). done. } *)
-(*     setoid_rewrite pred_at_sum in Hex'. rewrite Heq' in Hex'. *)
-(*     have Hpa: pred_at extr n (λ c _, locale_enabled ζ c). *)
-(*     { unfold pred_at. rewrite Heq'. destruct tr1'; eauto. } *)
-(*     destruct (Hex' Hpa) as [m Hm]. *)
-(*     have ?: infinite_trace tr1'. *)
-(*     { have Hinf := infinite_trace_after n extr Hinfin. by rewrite Heq' in Hinf. } *)
-(*     eapply (fairness_preserved_ind ρ _ f m ζ _ tr); eauto. *)
-(*     intros ?. by eapply fair_ex_after. *)
-(*   Qed. *)
-
-(*   Tactic Notation "inv" open_constr(P) := match goal with *)
-(*                 | [H: P |- _] => inversion H; clear H; simplify_eq *)
-(*                                           end. *)
-
-(* End fairness_preserved. *)
-
-Section fuel_dec_unless.
-  Context `{LM: LiveModel G Mdl LSI}.
-  Context `{Countable G}.
-  
-  Lemma fuel_must_not_incr_fuels oρ'
-    (δ1 δ2: LiveState G Mdl LSI)
-    ρ f1 f2
-    (KEEP: fuel_must_not_incr oρ' δ1 δ2)
-    (FUEL1: ls_fuel δ1 !! ρ = Some f1)
-    (FUEL2: ls_fuel δ2 !! ρ = Some f2)
-    (OTHER: oρ' ≠ Some ρ):
-    f2 <= f1.
-  Proof.
-    red in KEEP. specialize (KEEP ρ ltac:(by apply elem_of_dom)).
-    destruct KEEP as [LE|[?|KEEP]].
-    + rewrite FUEL1 FUEL2 in LE. simpl in LE. lia. 
-    + tauto. 
-    + apply proj1 in KEEP. destruct KEEP. eapply elem_of_dom; eauto.
-  Qed.
-
-  Lemma step_nonincr_fuels ℓ
-    (δ1 δ2: LiveState G Mdl LSI)
-    ρ f1 f2
-    (STEP: lm_ls_trans LM δ1 ℓ δ2)
-    (FUEL1: ls_fuel δ1 !! ρ = Some f1)
-    (FUEL2: ls_fuel δ2 !! ρ = Some f2)
-    (OTHER: forall g, ℓ ≠ Take_step ρ g):
-    f2 <= f1.
-  Proof.
-    destruct ℓ. 
-    all: eapply fuel_must_not_incr_fuels; eauto; [apply STEP|..]; congruence.
-  Qed. 
-
-
-  (* Definition Ul (ℓ: LM.(mlabel)) := *)
-  (*   match ℓ with *)
-  (*   | Take_step ρ _ => Some (Some ρ) *)
-  (*   | _ => None *)
-  (*   end. *)
-
-  Definition Usls (δ1: lm_ls LM) (ℓ: mlabel LM) (_: lm_ls LM):
-    option $ option $ fmrole Mdl :=
-    match ℓ with
-    | Take_step ρ _ => Some $ Some ρ
-    | _ => None
-    end.
-
-  Definition Ψ (δ: LiveState G Mdl LSI) :=
-    size δ.(ls_fuel) + [^ Nat.add map] ρ ↦ f ∈ δ.(ls_fuel (G := G)), f.
-
-  Lemma fuel_dec_unless (auxtr: auxtrace (LM := LM)) :
-    auxtrace_valid auxtr ->
-    dec_unless ls_under Usls Ψ auxtr.
-  Proof.
-    intros Hval n. revert auxtr Hval. induction n; intros auxtr Hval; last first.
-    { edestruct (after (S n) auxtr) as [auxtrn|] eqn:Heq; rewrite Heq =>//.
-      simpl in Heq;
-      simplify_eq. destruct auxtrn as [|δ ℓ auxtr']=>//; last first.
-      inversion Hval as [|???? Hmatch]; simplify_eq =>//.
-      specialize (IHn _ Hmatch). rewrite Heq // in IHn. }
-    edestruct (after 0 auxtr) as [auxtrn|] eqn:Heq; rewrite Heq =>//.
-    simpl in Heq; simplify_eq. destruct auxtrn as [|δ ℓ auxtr']=>//; last first.
-
-    inversion Hval as [|??? Htrans Hmatch]; simplify_eq =>//.
-    destruct ℓ as [| tid' |];
-      [left; eexists; done| right | inversion Htrans; naive_solver ].
-    destruct Htrans as (Hne&Hdec&Hni&Hincl&Heq). rewrite -> Heq in *. split; last done.
-
-    destruct (decide (dom $ ls_fuel δ = dom $ ls_fuel (trfirst auxtr'))) as [Hdomeq|Hdomneq].
-    - destruct Hne as [ρ Hρtid].
-
-      assert (ρ ∈ dom $ ls_fuel δ) as Hin by rewrite -ls_same_doms elem_of_dom //.
-      pose proof Hin as Hin'. pose proof Hin as Hin''.
-      apply elem_of_dom in Hin as [f Hf].
-      rewrite Hdomeq in Hin'. apply elem_of_dom in Hin' as [f' Hf'].
-      rewrite /Ψ -!size_dom Hdomeq.
-      apply Nat.add_lt_mono_l.
-
-      rewrite /Ψ (big_opM_delete (λ _ f, f) (ls_fuel (trfirst _)) ρ) //.
-      rewrite (big_opM_delete (λ _ f, f) (ls_fuel  δ) ρ) //.
-      apply Nat.add_lt_le_mono.
-      { rewrite /fuel_decr in Hdec. specialize (Hdec ρ). rewrite Hf Hf' /= in Hdec.
-        apply Hdec; [set_solver | set_solver | by econstructor]. }
-
-      apply big_addM_leq_forall => ρ' Hρ'.
-      rewrite dom_delete_L in Hρ'.
-      have Hρneqρ' : ρ ≠ ρ' by set_solver.
-      rewrite !lookup_delete_ne //.
-      destruct (decide (ρ' ∈ dom δ.(ls_fuel))) as [Hin|Hnotin]; last set_solver.
-      rewrite /fuel_must_not_incr in Hni.
-      (* destruct (Hni ρ' ltac:(done) ltac:(done)); [done|set_solver]. *)
-      destruct (Hni ρ' ltac:(done)); [done|set_solver].
-    - assert (size $ ls_fuel (trfirst auxtr') < size $ ls_fuel δ).
-      { rewrite -!size_dom. apply subset_size. set_solver. }
-      apply Nat.add_lt_le_mono =>//.
-      apply big_addM_leq_forall => ρ' Hρ'.
-      (* destruct (Hni ρ' ltac:(set_solver) ltac:(done)); [done|set_solver]. *)
-      destruct (Hni ρ' ltac:(set_solver)); [done|set_solver].
-  Qed.
-
-End fuel_dec_unless.
-
-Section destuttering_auxtr.
-  Context `{LM: LiveModel G M LSI}.
-
-  Context `{Countable G}.
-
-  (* Why is [LM] needed here? *)
-  Definition upto_stutter_auxtr :=
-    upto_stutter (ls_under (G:=G) (M:=M) (LSI := LSI)) (Usls (LM := LM)).
-
-  Lemma can_destutter_auxtr auxtr:
-    auxtrace_valid auxtr →
-    ∃ mtr, upto_stutter_auxtr auxtr mtr.
-  Proof.
-    intros ?. eapply can_destutter.
-    eapply fuel_dec_unless =>//.
-  Qed.
-
-End destuttering_auxtr.
-
-Section upto_preserves.
-  Context `{LM: LiveModel G M LSI}.
-  Context `{Countable G}.
-
-  Lemma upto_stutter_mono' :
-    monotone2 (upto_stutter_ind (ls_under (LSI := LSI)) (Usls (LM:=LM))).
-  Proof.
-    unfold monotone2. intros x0 x1 r r' IN LE.
-    induction IN; try (econstructor; eauto; done).
-  Qed.
-  Hint Resolve upto_stutter_mono' : paco.
-
-  Lemma upto_preserves_validity (auxtr : auxtrace (LM := LM)) mtr:
-    upto_stutter_auxtr auxtr mtr ->
-    auxtrace_valid auxtr ->
-    mtrace_valid mtr.
-  Proof.
-    revert auxtr mtr. pcofix CH. intros auxtr mtr Hupto Hval.
-    punfold Hupto.
-    induction Hupto as [| |btr str δ ????? IH].
-    - pfold. constructor.
-    - apply IHHupto. inversion Hval. assumption.
-    - pfold; constructor=>//.
-      + subst. inversion Hval as [| A B C Htrans E F ] =>//. subst. unfold ls_trans in *.
-        destruct ℓ; try done. simpl in *. simplify_eq.
-        destruct Htrans as [??].
-        have <- //: ls_under $ trfirst btr = trfirst str.
-        destruct IH as [IH|]; last done. punfold IH. inversion IH =>//.
-      + right. eapply CH.
-        { destruct IH =>//. }
-        subst. by inversion Hval.
-  Qed.
-
-End upto_preserves.
-
-Section upto_stutter_preserves_fairness_and_termination.
-  Context `{LM: LiveModel G M LSI}.
-  Context `{Countable G}.
-
-  Notation upto_stutter_aux := (upto_stutter (ls_under (LSI := LSI)) (Usls (LM := LM))).
-
-  Lemma upto_stutter_mono'' : (* TODO fix this proliferation *)
-    monotone2 (upto_stutter_ind (ls_under (LSI := LSI)) (Usls (LM:=LM))).
-  Proof.
-    unfold monotone2. intros x0 x1 r r' IN LE.
-    induction IN; try (econstructor; eauto; done).
-  Qed.
-  Hint Resolve upto_stutter_mono' : paco.
-
-  (* TODO: move *)
-  Lemma trace_lookup_0_singleton {St L: Type} (s: St):    
-    trace_lookup 0 (⟨ s ⟩: trace St L) = Some (s, None).
-  Proof. done. Qed. 
-
-  (* TODO: move *)
-  Lemma trace_lookup_0 {St L: Type} (tr: trace St L):    
-    exists ostep, trace_lookup 0 tr = Some (trfirst tr, ostep).
-  Proof.
-    rewrite /trace_lookup. rewrite after_0_id.
-    destruct tr; eauto. 
-  Qed.
-
-  Lemma upto_stutter_step_correspondence auxtr (mtr: mtrace M)
-    (Po: lm_ls LM -> option (mlabel LM * lm_ls LM) -> Prop)
-    (Pi: M -> option (option (fmrole M) * M) -> Prop)
-    (LIFT: forall δ ostep, Po δ ostep -> Pi (ls_under δ) (match ostep with 
-                                              | Some (ℓ, δ') => match (Usls δ ℓ δ') with | Some r => Some (r, ls_under δ') | None => None end
-                                              | None => None
-                                              end))
-    (PI0: forall st, Pi st None -> forall ℓ, Pi st (Some ℓ))
-    :
-    upto_stutter_auxtr auxtr mtr (LM := LM) ->
-    forall n atr_aux so stepo,
-      after n auxtr = Some atr_aux ->
-      (* pred_at atr_aux 0 Po -> *)
-      atr_aux !! 0 = Some (so, stepo) ->
-      Po so stepo ->
-    exists m atr_m si stepi,
-      after m mtr = Some atr_m /\ 
-      (* pred_at atr_m 0 Pi /\  *)
-      atr_m !! 0 = Some (si, stepi) /\
-      Pi si stepi /\
-      upto_stutter_auxtr atr_aux atr_m.
-  Proof.
-    intros Hupto n. generalize dependent auxtr. generalize dependent mtr. 
-    induction n as [|n]; intros auxtr mtr Hupto atr_aux os ostep AFTER O0 A0.
-    - rewrite after_0_id in AFTER. assert (atr_aux = mtr) as -> by congruence.
-      (* do 4 eexists. *)
-      exists 0, auxtr.
-      pose proof (trace_lookup_0 auxtr) as [stepi STEPI].
-      exists (trfirst auxtr), stepi.
-      do 3 (split; eauto). 
-      punfold Hupto. inversion Hupto; simplify_eq.
-      + rename A0 into Hpa.
-        rewrite /pred_at /=. rewrite /pred_at //= in Hpa.
-        destruct ostep; [done| ].
-        specialize (LIFT _ _ Hpa). simpl in LIFT.
-        simpl in O0. rewrite trace_lookup_0_singleton in O0, STEPI. 
-        rewrite trace_lookup_0_singleton in STEPI. 
-        congruence. 
-      +
-        (* rewrite -> !pred_at_0 in A0. *)
-        rewrite /pred_at /=.
-        destruct auxtr; try congruence.
-        * apply LIFT in A0. 
-          simpl.
-          rewrite trace_lookup_0_singleton in STEPI. inversion STEPI.
-          subst.           
-          rewrite trace_lookup_0_cons in O0. inversion O0. subst.
-          rewrite H0 in A0. congruence. 
-        * apply LIFT in A0.
-          simpl in H2. subst.
-          rewrite trace_lookup_0_cons in O0.
-          inversion O0. subst. simpl. 
-          rewrite H0 in A0.
-          destruct stepi; eauto. 
-      + 
-        (* rewrite -> !pred_at_0 in A0. *)
-        simpl. 
-        (* apply pred_at_0. rewrite <- H1. *)
-        eapply LIFT in A0.
-        rewrite trace_lookup_0_cons in O0. inversion O0. subst.
-        rewrite H1 in A0.
-        simpl in STEPI.
-        pose proof (trace_lookup_0_cons (ls_under os) ℓ' str).
-        simpl in H0. rewrite STEPI in H0. inversion H0. subst.
-        red in H2. try pclearbot.
-        apply upto_stutter_trfirst in H2. by rewrite H2.
-    - punfold Hupto. inversion Hupto as [| |?????? ?? IH ]; simplify_eq.
-      + simpl in AFTER. 
-        eapply IHn; eauto.
-        by pfold.
-      + simpl in AFTER.
-        assert (upto_stutter_auxtr btr str) as UPTO'.
-        { inversion IH; eauto. done. } 
-        specialize (IHn str btr UPTO').
-        specialize (IHn _ os ostep AFTER O0 A0). 
-        destruct IHn as (m&?&?&?&?&?&?&?). 
-        exists (S m). do 3 eexists. eauto. 
-  Qed.
-
-  (* Lemma upto_stutter_fairness_0 ρ auxtr (mtr: mtrace M): *)
-  (*   upto_stutter_aux auxtr mtr -> *)
-  (*   (* role_enabled_model ρ (trfirst mtr) -> *) *)
-  (*   (∃ n, pred_at auxtr n (λ δ _, ¬role_enabled (G := G) ρ δ) *)
-  (*         ∨ pred_at auxtr n (λ _ ℓ, ∃ ζ, ℓ = Some (Take_step ρ ζ))) -> *)
-  (*   ∃ m, pred_at mtr m (λ δ _, ¬role_enabled_model ρ δ) *)
-  (*        ∨ pred_at mtr m (λ _ ℓ, ℓ = Some $ Some ρ). *)
-  (*   Proof. *)
-  (*     intros Hupto (* Hre *) [n Hstep]. *)
-  (*     revert auxtr mtr Hupto (* Hre *) Hstep. *)
-  (*     induction n as [|n]; intros auxtr mtr Hupto (* Hre *) Hstep. *)
-  (*     - punfold Hupto. inversion Hupto; simplify_eq. *)
-  (*       + destruct Hstep as [Hpa|[??]]; try done. *)
-  (*         exists 0. left. rewrite /pred_at /=. rewrite /pred_at //= in Hpa. *)
-  (*       + rewrite -> !pred_at_0 in Hstep. exists 0. *)
-  (*         destruct Hstep as [Hstep| [tid Hstep]]; [left|right]. *)
-  (*         * rewrite /pred_at /=. destruct mtr; simpl in *; try congruence. *)
-  (*         * exfalso. injection Hstep => Heq. rewrite -> Heq in *. *)
-  (*           unfold Ul in *. congruence. *)
-  (*       + rewrite -> !pred_at_0 in Hstep. exists 0. *)
-  (*         destruct Hstep as [Hstep| [tid Hstep]]; [left|right]. *)
-  (*         * rewrite /pred_at //=. *)
-  (*         * rewrite /pred_at //=. injection Hstep. intros Heq. simplify_eq. *)
-  (*           unfold Ul in *. congruence. *)
-  (*     - punfold Hupto. inversion Hupto as [| |?????? ?? IH ]; simplify_eq. *)
-  (*       + destruct Hstep as [?|?]; done. *)
-  (*       + rewrite -> !pred_at_S in Hstep. *)
-  (*         eapply IHn; eauto. *)
-  (*         by pfold. *)
-  (*       + destruct (decide (ℓ' = Some ρ)). *)
-  (*         * simplify_eq. *)
-  (*           exists 0. right. rewrite pred_at_0 //. *)
-  (*         * have Hw: ∀ (P: nat -> Prop), (∃ n, P (S n)) -> (∃ n, P n). *)
-  (*           { intros P [x ?]. by exists (S x). } *)
-  (*           apply Hw. setoid_rewrite pred_at_S. *)
-  (*           eapply IHn; eauto. *)
-  (*           { destruct IH as [|]; done. } *)
-  (*   Qed. *)
-
-
-  Lemma upto_stutter_fairness_0 ρ auxtr (mtr: mtrace M):
-    upto_stutter_aux auxtr mtr ->
-    (∃ n, pred_at auxtr n (λ δ _, ¬role_enabled (LSI := LSI) ρ δ)
-          ∨ pred_at auxtr n (λ _ ℓ, ∃ ζ, ℓ = Some (Take_step ρ ζ))) ->
-    ∃ m, pred_at mtr m (λ δ _, ¬role_enabled_model ρ δ)
-         ∨ pred_at mtr m (λ _ ℓ, ℓ = Some $ Some ρ).
-  Proof.
-    repeat setoid_rewrite <- pred_at_or. 
-    intros UPTO [n NTH].
-    pose proof NTH as [atr AFTER]%pred_at_after_is_Some. 
-    rewrite (plus_n_O n) in NTH. 
-    rewrite pred_at_sum AFTER in NTH.
-    apply pred_at_trace_lookup' in NTH as (so & stepo & A0 & PROP).
-    pattern so, stepo in PROP. 
-    
-    eapply upto_stutter_step_correspondence in PROP; eauto. 
-    - destruct PROP as (m & atr_m & si & stepi & AFTERm & B0 & Pi & UPTO').
-      exists m. rewrite (plus_n_O m) pred_at_sum AFTERm.
-      eapply pred_at_trace_lookup'.
-      do 2 eexists. split; [eauto| ].
-      pattern si. pattern stepi. apply Pi. 
-    - intros ?? Po. simpl. destruct Po as [?| ?]; eauto.
-      right. destruct H0 as [? H0].
-      destruct ostep; try done. simpl in *.
-      destruct p. simpl in H0. inversion H0. by subst.
-    - intros. destruct H0; [| done]. eauto.
-  Qed.  
-    
-  Lemma upto_stutter_fairness (auxtr:auxtrace (LM := LM)) (mtr: mtrace M):
-    upto_stutter_aux auxtr mtr ->
-    (∀ ρ, fair_aux ρ auxtr) ->
-    (∀ ρ, fair_model_trace ρ mtr).
-  Proof.
-    intros Hupto Hfa ρ n Hpmod.
-    unfold pred_at in Hpmod.
-    destruct (after n mtr) as [mtr'|] eqn:Heq; last done.
-    destruct (upto_stutter_after _ _ n Hupto Heq) as (n'&auxtr'&Heq'&Hupto').
-    have Hre: role_enabled_model ρ (trfirst mtr') by destruct mtr'.
-    specialize (Hfa ρ).
-    have Henaux : role_enabled ρ (trfirst auxtr').
-    { have HUs: ls_under (trfirst auxtr') = trfirst mtr'.
-      - punfold Hupto'. by inversion Hupto'.
-      - unfold role_enabled, role_enabled_model in *.
-        rewrite HUs //. }
-    (* have Hfa' := (fair_by_after ρ auxtr n' auxtr' Hfa Heq' 0). *)
-    have Hfa' := (fair_by_after _ _ ρ auxtr auxtr' n' Heq' Hfa 0).
-    
-    have Hpredat: pred_at auxtr' 0 (λ δ _, role_enabled ρ δ).
-    { rewrite /pred_at /=. destruct auxtr'; done. }
-
-    specialize (Hfa' Hpredat). clear Hpredat.
-    destruct Hfa' as (m&Hres). simpl in Hres.
-    (* rewrite /fairness_sat.  *)
-    repeat setoid_rewrite pred_at_sum. rewrite !Heq. rewrite /role_match. 
-    setoid_rewrite pred_at_iff.
-    2: { intros. apply Morphisms_Prop.or_iff_morphism; [reflexivity| ].
-         Unshelve. 2: exact (ol = Some (Some ρ)).
-         split; [intros (?&->&->)| intros ->]; eauto. }
-    setoid_rewrite pred_at_or. 
-    eapply upto_stutter_fairness_0; eauto.
-    eexists. rewrite -pred_at_or.
-    eapply pred_at_iff; eauto. intros.
-    apply Morphisms_Prop.or_iff_morphism; [done| ].
-    rewrite /lbl_with_role. split; [intros (?&->)| intros (?&->&(?&->))]; eauto. 
-  Qed.
-
-  Lemma upto_stutter_finiteness auxtr (mtr: mtrace M):
-    upto_stutter_aux auxtr mtr ->
-    terminating_trace mtr ->
-    terminating_trace auxtr.
-  Proof.
-    intros Hupto [n Hfin].
-    have [n' ?] := upto_stutter_after_None _ _ n Hupto Hfin.
-    eexists; done.
-  Qed.
-
-End upto_stutter_preserves_fairness_and_termination.
