fairness/lm_fairness_preservation.v
@@ -1,22 +1,25 @@
 From stdpp Require Import option.
 From Paco Require Import paco1 paco2 pacotac.
 From trillium.program_logic Require Export adequacy.
-From trillium.fairness Require Export inftraces fairness fuel traces_match trace_utils.
-From trillium.fairness Require Import lm_fair. (* TODO: remove? it's only for lm_lbl_matches_group *)
+From trillium.fairness Require Export inftraces fairness fuel traces_match trace_utils lm_fair_traces lm_fair trace_helpers trace_lookup. 
 
 
 Section fairness_preserved.
   Context `{LM: LiveModel G M LSI}.
-  Context `{EqDecision G}.
+  (* Context `{EqDecision G}. *)
+  Context {LF: LMFairPre LM}. 
 
   Lemma mapping_live_role (δ: LiveState G M LSI) ρ:
     ρ ∈ M.(live_roles) δ ->
     is_Some (ls_mapping δ !! ρ).
-  Proof. rewrite -elem_of_dom ls_same_doms. SS. Qed.
+  Proof. by intros ?%ls_mapping_dom%elem_of_dom. Qed.
   Lemma fuel_live_role (δ: LiveState G M LSI) ρ:
     ρ ∈ M.(live_roles) δ ->
     is_Some (ls_fuel δ !! ρ).
-  Proof. rewrite -elem_of_dom. SS. Qed.
+  Proof. 
+    intros ?%ls_mapping_dom.
+    apply elem_of_dom. by rewrite -ls_same_doms.
+  Qed. 
 
   Local Hint Resolve mapping_live_role: core.
   Local Hint Resolve fuel_live_role: core.
@@ -28,67 +31,48 @@ Section fairness_preserved.
   (* Definition group_step_or_dis *)
   (*   (τ: G) (δ: LiveState G M LSI) (oℓ: option (lm_lbl LM)) := *)
   (*   (forall ρ, ¬ ls_mapping δ !! ρ = Some τ) \/ (∃ ℓ, oℓ = Some ℓ /\ lm_lbl_matches_group ℓ τ). *)
-  Definition group_step_or_dis (τ: G) (δ: LiveState G M LSI) (oℓ: option (lm_lbl LM)) :=
-    fairness_sat (λ τ δ, exists ρ, ls_mapping δ !! ρ = Some τ) (flip lm_lbl_matches_group) τ δ oℓ.
+  Definition group_step_or_dis (τ: G) (δ: LiveState G M LSI) (og: option $ option G) :=
+    fairness_sat (λ τ δ, exists ρ, ls_mapping δ !! ρ = Some τ) (fun t og' => og' = Some t) τ δ og.
 
-  Definition fair_by_group: G -> auxtrace (LM := LM) -> Prop := 
+  Definition fair_by_group: G -> lmftrace (LM := LM) -> Prop := 
     fair_by (λ τ δ, exists ρ, ls_mapping δ !! ρ = Some τ)
-      (flip lm_lbl_matches_group). 
+      (fun t og' => og' = Some t). 
   
   (* Definition steps_or_unassigned *)
   (*   (ρ: fmrole M) (δ: LiveState G M LSI) (ℓ: option (lm_lbl LM)) := *)
   (*   (∀ τ, ls_mapping δ !! ρ ≠ Some τ) \/ (∃ τ, ℓ = Some $ Take_step ρ τ). *)
-  Definition steps_or_unassigned
-    (ρ: fmrole M) (δ: LiveState G M LSI) (oℓ: option (lm_lbl LM)) :=
-    fairness_sat (λ ρ δ, ρ ∈ dom (ls_mapping δ))
-      (fun ρ ℓ => exists τ, ℓ = Take_step ρ τ) ρ δ oℓ.
+  Definition steps_or_unassigned :=
+    fairness_sat_gen (λ ρ δ, ρ ∈ dom (ls_mapping δ)) step_by_next_TS.
     
-  Definition fair_aux_SoU: fmrole M -> auxtrace (LM := LM) -> Prop := 
-    fair_by (λ ρ δ, ρ ∈ dom (ls_mapping δ))
-      (fun ρ ℓ => exists τ, ℓ = Take_step ρ τ). 
+  Definition fair_aux_SoU: fmrole M -> lmftrace (LM := LM) -> Prop := 
+    fair_by_gen (λ ρ δ, ρ ∈ dom (ls_mapping δ))
+      step_by_next_TS. 
 
-  (* (* TODO: ? try to unify with fair_aux_after *) *)
-  (* (* TODO: add ∀ in fair_aux_SoU definition  *) *)
-  (* Lemma fair_aux_SoU_after ρ (auxtr: auxtrace (LM := LM)) *)
-  (*   n auxtr': *)
-  (*   (forall k, fair_aux_SoU auxtr ρ k) -> *)
-  (*   after n auxtr = Some auxtr' -> *)
-  (*   (forall k, fair_aux_SoU auxtr' ρ k). *)
-  (* Proof. *)
-  (*   rewrite /fair_aux_SoU => Hfair Hafter m Hpa. *)
-  (*   specialize (Hfair (n+m)). *)
-  (*   rewrite -> (pred_at_sum _ n) in Hfair. rewrite Hafter in Hfair. *)
-  (*   destruct (Hfair Hpa) as (p&Hp). *)
-  (*   exists (p). *)
-  (*   rewrite <-Nat.add_assoc, ->!(pred_at_sum _ n) in Hp. *)
-  (*   by rewrite Hafter in Hp.  *)
-  (* Qed. *)
-
-  Definition fairness_induction_stmt ρ fm f m τ (* extr *) (auxtr : auxtrace (LM := LM)) δ
+  Definition fairness_induction_stmt ρ fm f m τ (* extr *) (auxtr : lmftrace (LM := LM)) δ
     :=
-      (
-        infinite_trace auxtr ->
-          (forall τ, fair_by_group τ auxtr) ->
-       fm = (f, m) ->
-       δ = trfirst auxtr ->
-       δ.(ls_fuel) !! ρ = Some f ->
-       δ.(ls_mapping) !! ρ = Some τ ->
-       pred_at auxtr m (fun δ oℓ => group_step_or_dis τ δ oℓ)
-       ->
-      ∃ M, pred_at auxtr M (fun δ ℓ => steps_or_unassigned ρ δ ℓ)). 
+    infinite_trace auxtr ->
+    (forall τ, fair_by_group τ auxtr) ->
+    fm = (f, m) ->
+    δ = trfirst auxtr ->
+    δ.(ls_fuel) !! ρ = Some f ->
+    δ.(ls_mapping) !! ρ = Some τ ->
+    pred_at auxtr m (fun δ oℓ => group_step_or_dis τ δ oℓ)
+    ->
+    (* ∃ M, pred_at auxtr M (fun δ ℓ => steps_or_unassigned ρ δ ℓ)).  *)
+    exists i δi ostep, auxtr !! i = Some (δi, ostep) /\ steps_or_unassigned ρ δi ostep.
   
-  Local Lemma case1 ρ f m (auxtr' : auxtrace (LM := LM)) δ ℓ :
+  Local Lemma case1 ρ f m (auxtr' : lmftrace (LM := LM)) δ ℓ :
     (∀ m0 : nat * nat,
          strict lt_lex m0 (f, m)
-         → ∀ (f m: nat) τ (auxtr : auxtrace (LM := LM))
+         → ∀ (f m: nat) τ (auxtr : lmftrace (LM := LM))
              (δ : LiveState G M LSI),
-          auxtrace_valid auxtr -> fairness_induction_stmt ρ m0 f m τ (* extr *) auxtr δ ) ->
+          mtrace_valid auxtr -> fairness_induction_stmt ρ m0 f m τ (* extr *) auxtr δ ) ->
     (ρ ∈ dom (ls_fuel (trfirst auxtr')) → oless (ls_fuel (trfirst auxtr') !! ρ) (ls_fuel δ !! ρ)) ->
-    auxtrace_valid auxtr' ->
+    mtrace_valid auxtr' ->
     infinite_trace auxtr' ->
     ls_fuel δ !! ρ = Some f ->
     (forall τ, fair_by_group τ auxtr' ) ->
-    ∃ M0 : nat, pred_at (δ -[ ℓ ]-> auxtr') M0 (fun δ ℓ => steps_or_unassigned ρ δ ℓ).
+    ∃ i δi ostep, (δ -[ ℓ ]-> auxtr') !! i = Some (δi, ostep) /\ steps_or_unassigned ρ δi ostep.
   Proof.
       intros IH Hdec (* Hmatch *) Hvalid Hinf Hsome Hfair.
       unfold oless in Hdec.
@@ -97,112 +81,30 @@ Section fairness_preserved.
       destruct (ls_fuel (trfirst auxtr') !! ρ) as [f'|] eqn:Heq.
       -
         destruct (decide (exists τ, ls_mapping (trfirst auxtr') !! ρ = Some τ)) as [MAP| ]; last first.
-        { exists 1. apply pred_at_S.
-          rewrite /steps_or_unassigned. apply pred_at_or. left.
-          eapply pred_at_state_trfirst. intros ?%elem_of_dom. eauto. }
+        { exists 1. rewrite trace_lookup_cons.
+          pose proof (trace_lookup_0 auxtr') as (?&?).
+          do 2 eexists. split; eauto. 
+          rewrite /steps_or_unassigned. left.
+          intros ?%elem_of_dom. apply n. done. }
         destruct MAP as [τ' Hτ']. 
         pose proof (Hfair τ' 0) as [p Hp]. 
         { rewrite pred_at_state_trfirst. eauto. } 
 
-        have [P Hind] : ∃ M0 : nat, pred_at auxtr' M0 (steps_or_unassigned ρ).
-        { red in Hp. simpl in Hp. 
-          eapply (IH _ _ _ p _); eauto.
-          Unshelve. unfold strict, lt_lex. specialize (Hdec ltac:(by eapply elem_of_dom_2)).
-          lia. }
-        exists (1+P). rewrite !pred_at_sum. simpl. done.
-      - exists 1. apply pred_at_S.
-        rewrite /steps_or_unassigned. apply pred_at_or. left.
-        apply pred_at_state_trfirst.
-        by rewrite -ls_same_doms in Hdec.
-  Qed.
-  
-  Local Ltac SS' := eapply elem_of_dom; eauto. 
-  
-  (* TODO: use this lemma in other places *)
-  Lemma others_step_fuel_decr ρ f f' τ
-    δ ℓ δ'
-    (STEP: lm_ls_trans LM δ ℓ δ')
-    (Hfuel : ls_fuel δ !! ρ = Some f)
-    (Hmapping : ls_mapping δ !! ρ = Some τ)
-    (Hζ: ¬ lm_lbl_matches_group ℓ τ (LM := LM))
-    (FUEL: ls_fuel δ' !! ρ = Some f'):
-    f' ≤ f.
-  Proof.
-    simpl in *. destruct ℓ as [ρ0 ζ0| ζ0|]; try done.
-    + destruct STEP as (?&?&?&Hnoninc&?).
-      unfold fuel_must_not_incr in Hnoninc.
-      have Hneq: Some ρ ≠ Some ρ0 by congruence.
-      specialize (Hnoninc ρ ltac:(SS')).
-      unfold oleq in Hnoninc. rewrite Hfuel in Hnoninc.
-      rewrite FUEL in Hnoninc.
-      destruct Hnoninc as [?|[?|C]]. 
-      3: { destruct (proj1 C). eapply elem_of_dom; eauto. }
-      all: set_solver. 
-    + destruct STEP as (?&?&Hnoninc&?).
-      unfold fuel_must_not_incr in Hnoninc.
-      have Hneq: Some ρ ≠ None by congruence.
-      specialize (Hnoninc ρ ltac:(SS')).
-      unfold oleq in Hnoninc. rewrite Hfuel in Hnoninc.
-      rewrite FUEL in Hnoninc. 
-      destruct Hnoninc as [?|[?|C]]. 
-      3: { destruct (proj1 C). eapply elem_of_dom; eauto. }
-      all: set_solver.
-    + destruct STEP as [_ [_ [Hnoninc _]]].
-      have HnotNone: Some ρ ≠ None by congruence.
-      specialize (Hnoninc ρ ltac:(SS')).
-      unfold oleq in Hnoninc. rewrite Hfuel in Hnoninc.
-      rewrite FUEL in Hnoninc. 
-      destruct Hnoninc as [?|[?|C]]. 
-      3: { destruct (proj1 C). eapply elem_of_dom; eauto. }
-      all: set_solver.
-  Qed. 
-  
-  (* TODO: use this lemma in other places *)
-  Lemma owner_change_fuel_decr ρ f f'
-    δ ℓ δ'
-    τ τ''
-    (STEP: lm_ls_trans LM δ ℓ δ')
-    (Hfuel: ls_fuel δ !! ρ = Some f)
-    (Hmapping: ls_mapping δ !! ρ = Some τ)
-    (Hζ'' : ls_mapping δ' !! ρ = Some τ'')
-    (Hchange : τ ≠ τ'')
-    (FUEL: ls_fuel δ' !! ρ = Some f'):
-    f' < f.
-  Proof.
-    destruct ℓ as [ρ0 ζ0| ζ0|]; try done.
-    + destruct STEP as (?&?&Hdec&?&?).
-      unfold fuel_decr in Hdec. simplify_eq.
-      have Hmd: must_decrease ρ (Some ρ0) δ δ' (Some ζ0).
-      { econstructor 2. congruence. rewrite Hζ''; eauto. }
-      specialize (Hdec ρ ltac:(SS') ltac:(SS') Hmd).
-      unfold oleq in Hdec. rewrite Hfuel in Hdec.
-      by rewrite FUEL in Hdec. 
-    + destruct STEP as (?&Hdec&_).
-      unfold fuel_decr in Hdec. simplify_eq.
-      have Hmd: must_decrease ρ None δ δ' (Some ζ0).
-      { econstructor 2. congruence. rewrite Hζ''; eauto. }
-      specialize (Hdec ρ ltac:(SS') ltac:(SS') Hmd).
-      unfold oleq in Hdec. rewrite Hfuel in Hdec.
-      by rewrite FUEL in Hdec.
-    + destruct STEP as [_ [Hdec _]].
-      unfold fuel_decr in Hdec.
-      have Hmd: must_decrease ρ None δ δ' None.
-      { econstructor. congruence. rewrite Hζ''. eauto. }
-      specialize (Hdec ρ ltac:(SS') ltac:(SS') Hmd).
-      unfold oleq in Hdec. rewrite Hfuel in Hdec.
-      by rewrite FUEL in Hdec.
-  Qed.
-
-  (* TODO: move *)
-  Local Instance lm_lbl_match_Dec: 
-    forall ℓ τ, Decision (lm_lbl_matches_group ℓ τ (LM := LM)).
-  Proof.
-    intros. destruct ℓ; simpl; solve_decision.
+        assert (∃ i δi ostep, auxtr' !! i = Some (δi, ostep) /\ steps_or_unassigned ρ δi ostep) as (i&?&?&?&?). 
+        { eapply (IH _ _ _ p _); eauto.
+          Unshelve. 
+          unfold strict, lt_lex. specialize (Hdec ltac:(by eapply elem_of_dom_2)).
+          rewrite Heq in Hdec. lia. } 
+        exists (1+i). eauto. 
+      - pose proof (trace_lookup_0 auxtr') as (?&?).
+        exists 1. do 2 eexists. rewrite trace_lookup_cons. split; eauto. 
+        rewrite /steps_or_unassigned. left.
+        apply not_elem_of_dom in Heq. by rewrite -ls_same_doms in Heq. 
   Qed.
   
   Lemma fairness_preserved_ind ρ:
-    ∀ fm f m τ (auxtr: auxtrace (LM := LM)) δ,
-      auxtrace_valid auxtr -> 
+    ∀ fm f m τ (auxtr: lmftrace (LM := LM)) δ,
+      mtrace_valid auxtr -> 
       fairness_induction_stmt ρ fm f m τ auxtr δ.
   Proof.    
     induction fm as [fm IH] using lex_ind.
@@ -212,78 +114,84 @@ Section fairness_preserved.
     have Hfair': (forall τ, fair_by_group τ auxtr'). 
     { intros. eapply fair_by_cons; eauto. apply Hfair. }
     simpl in *. subst δ_. 
-    destruct (decide (lm_lbl_matches_group ℓ τ)) as [Hζ|Hζ].
-    - destruct ℓ; simpl in Hζ; try done; subst g; last first.       
-      + pose proof (auxtrace_valid_forall _ VALID 0) as Hls. 
-        simpl in Hls. 
-        destruct Hls as (? & Hlsdec & Hlsincr).
-        unfold fuel_decr in Hlsdec.
-        have Hmustdec: must_decrease ρ None δ (trfirst auxtr') (Some τ).
-        { constructor; eauto. }
-        eapply case1 =>//.
-        * move=> Hinfuel; apply Hlsdec => //; first set_solver.
-        * eapply auxtrace_valid_after with (n := 1); eauto. 
-        * eapply infinite_cons =>//.
+    (* destruct (decide (lm_lbl_matches_group ℓ τ)) as [Hζ|Hζ]. *)
+    destruct (decide (ℓ = Some τ)) as [Hζ|Hζ]. 
+    - subst.
+      (* pose proof (mtrace_valid_steps' VALID 0) as Hls.  *)
+      pose proof (mtrace_valid_cons _ _ _ VALID) as [_ Hls]. simpl in Hls.
+      destruct (next_TS_role δ τ (trfirst auxtr')) eqn:N. 
       + (* Three cases: *)
 (*            (1) ρ' = ρ and we are done *)
 (*            (2) ρ' ≠ ρ but they share the same ρ -> ρ decreases *)
 (*            (3) ρ' ≠ ρ and they don't have the same tid -> *)
 (*            impossible because tid and the label must match! *)
-        pose proof (auxtrace_valid_forall _ VALID 0) as Hls. 
-        simpl in Hls. 
+        clear Hls. 
+        pose proof N as Hls%next_TS_spec_pos. 
         destruct (decide (ρ = f0)) as [->|Hρneq].
-        { exists 0. right. rewrite /pred_at /=. eauto. }
+        { exists 0. do 2 eexists. rewrite trace_lookup_0_cons. split; eauto. 
+          right. red. eauto. }
         destruct Hls as (?&Hsame&Hdec&Hnotinc&_).
         rewrite -Hsame /= in Hmapping.
         have Hmustdec: must_decrease ρ (Some f0) δ (trfirst auxtr') (Some τ).
         { constructor; eauto; congruence. }
         (* Copy and paste begins here *)
         eapply case1 =>//; last by eauto using infinite_cons.
-        2: { eapply auxtrace_valid_after with (n := 1); eauto. }
+        2: { eapply mtrace_valid_cons; eauto. }
         intros Hinfuels. apply Hdec =>//. 
         clear -Hfuel. apply elem_of_dom; eauto.
-
+      + eapply next_TS_spec_inv_S in N; eauto. clear Hls. rename N into Hls.  
+        destruct Hls as (? & Hlsdec & Hlsincr).
+        unfold fuel_decr in Hlsdec.
+        have Hmustdec: must_decrease ρ None δ (trfirst auxtr') (Some τ).
+        { constructor; eauto. }
+        eapply case1 =>//.
+        * move=> Hinfuel; apply Hlsdec => //; first set_solver.
+        * eapply mtrace_valid_cons; eauto. 
+        * eapply infinite_cons =>//.
     - (* Another thread is taking a step. *)
       destruct (decide (exists τ, ls_mapping (trfirst auxtr') !! ρ = Some τ)) as [MAP| ]; last first.
-      { exists 1. apply pred_at_or. left.
-        eapply pred_at_state_trfirst; eauto.
-        by intros ?%elem_of_dom. }
+      { exists 1. pose proof (trace_lookup_0 auxtr') as (?&?). 
+        do 2 eexists. rewrite trace_lookup_cons. split; eauto.         
+        left. by intros ?%elem_of_dom. }
       destruct m as [| m'].
       { rewrite -> !pred_at_0 in Hexen.
         red in Hexen. destruct Hexen as [Hexen|Hexen].
-        -
-          exfalso. set_solver. 
+        - exfalso. set_solver. 
         - destruct Hexen as (?&?&?). set_solver. }
-      pose proof (auxtrace_valid_forall _ VALID 0) as Hls. simpl in Hls.
+      pose proof (mtrace_valid_cons _ _ _ VALID) as [_ Hls]. simpl in Hls.
+      destruct ℓ; [| done]. 
       destruct MAP as [τ'' Hτ'']. 
       destruct (ls_fuel (trfirst auxtr') !! ρ) as [f'| ] eqn:Hfuel'.
       2: { apply elem_of_dom_2 in Hτ''. apply not_elem_of_dom_2 in Hfuel'.
            rewrite ls_same_doms in Hτ''. done. }
+      red in Hls. destruct Hls as (ℓ & STEP & MATCH). 
       destruct (decide (τ = τ'')) as [<-|Hchange].
-      + assert (f' <= f) as Hff' by (eapply others_step_fuel_decr; eauto).
+      + assert (f' <= f) as Hff'.
+        { eapply others_step_fuel_decr; eauto.
+          destruct ℓ; simpl in *; congruence. }
         unfold fair_by in *.
-        have [P Hind] : ∃ M0 : nat, pred_at auxtr' M0 (steps_or_unassigned ρ).
+        assert (exists i δi ostep, auxtr' !! i = Some (δi, ostep) /\ steps_or_unassigned ρ δi ostep) as (P&?&?&Hind).
         { eapply (IH _ _ _ m' _); eauto.
-          - eapply auxtrace_valid_after with (n := 1); eauto.
+          - eapply mtrace_valid_cons; eauto.
           - by eapply infinite_cons.
           Unshelve. unfold strict, lt_lex. lia. }
-        exists (1+P). rewrite !pred_at_sum. simpl. done.
+        exists (1+P). eauto.
       + assert (f' < f) as Hff' by (eapply owner_change_fuel_decr; eauto). 
         unfold fair_by in *.
         pose proof (Hfair' τ'' 0) as [p Hp].
         { rewrite pred_at_state_trfirst. eauto. }        
-        have [P Hind] : ∃ M0 : nat, pred_at auxtr' M0 (steps_or_unassigned ρ).
+        assert (exists i δi ostep, auxtr' !! i = Some (δi, ostep) /\ steps_or_unassigned ρ δi ostep) as (P&?&?&Hind).
         { eapply (IH _ _ _ p _); eauto.
-          - eapply auxtrace_valid_after with (n := 1); eauto.
+          - eapply mtrace_valid_cons; eauto.
           - by eapply infinite_cons.
           Unshelve. unfold strict, lt_lex. lia. }
-        exists (1+P). rewrite !pred_at_sum. simpl. done.
+        exists (1+P). eauto.
   Qed.
   
   Lemma group_fairness_implies_step_or_unassign
-    (auxtr: auxtrace (LM := LM)):
+    (auxtr: lmftrace (LM := LM)):
     infinite_trace auxtr ->
-    auxtrace_valid auxtr ->
+    mtrace_valid auxtr ->
     (forall τ, fair_by_group τ auxtr) ->
     forall ρ, fair_aux_SoU ρ auxtr.
   Proof.
@@ -292,7 +200,8 @@ Section fairness_preserved.
     unfold pred_at in DOMn.
     destruct (after n auxtr) as [tr|] eqn:Heq; rewrite Heq in DOMn.
     2: { done. } 
-    setoid_rewrite pred_at_sum. rewrite Heq.
+    (* setoid_rewrite pred_at_sum. rewrite Heq. *)
+    setoid_rewrite <- trace_lookup_after; eauto.  
 
     have [τ Hτ] : is_Some((trfirst tr).(ls_mapping) !! ρ).
     { destruct tr; apply elem_of_dom; eauto. }
@@ -309,147 +218,172 @@ Section fairness_preserved.
     have ?: infinite_trace tr.
     { have Hinf := infinite_trace_after n auxtr Hinfin. by rewrite Heq in Hinf. }
     eapply (fairness_preserved_ind ρ _ f m τ _); eauto.
-    - eapply auxtrace_valid_after; eauto. 
+    - eapply trace_valid_after; eauto. 
     - intros. eapply fair_by_after; eauto. apply Hex. 
   Qed.
 
-  Lemma steps_or_unassigned_implies_aux_fairness (auxtr: auxtrace (LM := LM)):
-    (forall ρ, fair_aux_SoU ρ auxtr) -> (forall ρ, fair_aux ρ auxtr (LM := LM)).
+  (* TODO: move*)
+  Lemma pred_at_ex {S L T: Type} (P : T -> S → option L → Prop) tr n:
+    pred_at tr n (fun s ol => exists t, P t s ol) <-> exists t, pred_at tr n (P t).
+  Proof.
+    rewrite /pred_at. destruct after.
+    2: { intuition. by destruct H. }
+    destruct t; eauto.
+  Qed.     
+
+  Lemma steps_or_unassigned_implies_aux_fairness (auxtr: lmftrace (LM := LM)):
+    (forall ρ, fair_aux_SoU ρ auxtr) -> (forall ρ, fair_by_next_TS ρ auxtr).
   Proof.
     intros FAIR ρ n Hn.
     eapply pred_at_impl in Hn.
-    2: { intros ? ? EN%mapping_live_role%elem_of_dom. apply EN. }
-    specialize (FAIR _ _ Hn). destruct FAIR as (m & STEP).
-    exists m. eapply pred_at_impl; [| apply STEP].
-    rewrite /fairness_sat. intros. destruct H; eauto.
-    left. intros [??]%mapping_live_role. destruct H. by apply elem_of_dom.  
+    2: { intros ?? EN%mapping_live_role%elem_of_dom. apply EN. }
+    specialize (FAIR _ _ Hn).
+    destruct FAIR as (m&?&?&NMth&STEP).
+    exists m.
+    do 2 eexists. split; eauto. 
+    destruct STEP. 
+    - left. intros ?%mapping_live_role.
+      by apply H, elem_of_dom.
+    - by right.
   Qed.
 
-  Lemma group_fairness_implies_role_fairness (auxtr: auxtrace (LM := LM)):
+  Lemma group_fairness_implies_role_fairness (auxtr: lmftrace (LM := LM)):
     infinite_trace auxtr ->
-    auxtrace_valid auxtr ->
+    mtrace_valid auxtr ->
     (forall τ, fair_by_group τ auxtr) ->
-    (forall ρ, fair_aux ρ auxtr (LM := LM)).
+    (forall ρ, fair_by_next_TS ρ auxtr).
   Proof. 
     intros. auto using steps_or_unassigned_implies_aux_fairness, 
       group_fairness_implies_step_or_unassign.
   Qed. 
     
   Section Preservation.
-      Context {So Lo: Type}.
-      Context `{EqDecision Lo}. 
-
-      Let out_trace := trace So (option Lo).
-
-      (* counterpart of locale step.
-     TODO: any restrictions? *)
-      Context (out_step: So -> option Lo -> So -> Prop). 
-
-      (* Representation of group labels on outer level *)
-      Context (lift_grole: G -> Lo).
-      Hypothesis (INJlg: Inj eq eq lift_grole). 
-      
-      Context (locale_prop: Lo -> So -> Prop).
-
-      (* Context (state_rel: cfg Λ → lm_ls LM → Prop). *)
-      Context (state_rel: So → lm_ls LM → Prop).
-
-      Definition lm_live_lift := forall ζ ρ δ c,
-          ls_mapping δ !! ρ = Some ζ ->
-          (* ρ ∈ live_roles _ δ ->  *)
-          state_rel c δ ->
-          (* locale_enabled ζ c *)
-          locale_prop (lift_grole ζ) c. 
-
-
-      Hypothesis (match_locale_prop_states: lm_live_lift).
-
-      Definition out_LM_labels_match (oζ : option Lo) (ℓ: lm_lbl LM) :=
-        match oζ with
-        | Some ζ =>
-            exists τ, ζ = lift_grole τ /\
-                   match ℓ with
-                   | Take_step _ τ' | Silent_step τ' => τ = τ'
-                   | Config_step => False
-                   end
-        | None => match ℓ with
-                 | Config_step => True
-                 | _ => False
-                 end
-        end. 
-
-      (* TODO: rename *)
-      Definition lm_exaux_traces_match_gen: out_trace → auxtrace (LM := LM) → Prop :=
-        traces_match 
-          (* labels_match *) out_LM_labels_match
-          (* live_tids *) state_rel
-          (* locale_step  *) out_step
-          LM.(lm_ls_trans).
-
-      From trillium.fairness Require Import trace_lookup.
-
-      (* TODO: move *)
-      Lemma pred_at_impl {St L : Type} (P Q: St -> option L -> Prop)
-        (IMPL: forall s ol, P s ol -> Q s ol):
-        forall tr i, pred_at tr i P -> pred_at tr i Q.
-      Proof.
-        rewrite /pred_at. intros. 
-        destruct after; intuition; destruct t.
-        all: by apply IMPL.
-      Qed.
-
-      Let lbl_match (ℓ: Lo) oℓ' := oℓ' = Some ℓ. 
+    Context {So Lo: Type}.
+    Context `{EqDecision Lo}. 
     
-      Theorem fairness_preserved (extr: out_trace) (auxtr: auxtrace (LM := LM)):
-        infinite_trace extr ->
-        lm_exaux_traces_match_gen extr auxtr ->
-        (forall ζ, fair_by locale_prop lbl_match ζ extr) -> (forall τ, fair_by_group τ auxtr).
-      Proof.
-        intros INF MATCH FAIR_OUT.
-        intros. do 2 red. intros n ASG.
-        pose proof ASG as (δ & NTH & [ρ MAP])%pred_at_trace_lookup.
-        
-        edestruct @traces_match_state_lookup_2 as (c & ENTH & RELn); eauto.
-        
-        red in FAIR_OUT. edestruct FAIR_OUT as [m STEP].
-        { eapply pred_at_trace_lookup; eauto. }
-        apply pred_at_or in STEP.
-
-        apply pred_at_or in STEP. 
-        apply pred_at_trace_lookup in STEP as (c' & ENTH' & STEP).
-        edestruct @traces_match_state_lookup_1 as (δ' & NTH' & RELn'); eauto. 
-        exists m. apply pred_at_trace_lookup. eexists. split; eauto.
-        red. destruct STEP as [EMP | STEP]. 
-        - left. intros [??]. apply EMP. eapply match_locale_prop_states; eauto.  
-        - right.
-          destruct STEP as (?&?&LBLM). 
-          edestruct @traces_match_label_lookup_1 as (ℓ & NTH'l & LBL); eauto.
-          eexists. split; eauto. red in LBL.
-          red in LBLM. subst. 
-          destruct LBL as [? [->%INJlg ?]]. done. 
-      Qed.      
+    Let out_trace := trace So (option Lo).
+    
+    (* counterpart of locale step.
+       TODO: any restrictions? *)
+    Context (out_step: So -> option Lo -> So -> Prop). 
+    
+    (* Representation of group labels on outer level *)
+    Context (lift_grole: G -> Lo).
+    Hypothesis (INJlg: Inj eq eq lift_grole). 
+    
+    Context (locale_prop: Lo -> So -> Prop).
+    
+    (* Context (state_rel: cfg Λ → lm_ls LM → Prop). *)
+    Context (state_rel: So → lm_ls LM → Prop).
+    
+    Definition lm_live_lift := forall ζ ρ δ c,
+        ls_mapping δ !! ρ = Some ζ ->
+        (* ρ ∈ live_roles _ δ ->  *)
+        state_rel c δ ->
+        (* locale_enabled ζ c *)
+        locale_prop (lift_grole ζ) c. 
+    
+    
+    Hypothesis (match_locale_prop_states: lm_live_lift).
+    
+    (* Definition out_LM_labels_match (oζ : option Lo) (ℓ: lm_lbl LM) := *)
+    (*   match oζ with *)
+    (*   | Some ζ => *)
+    (*       exists τ, ζ = lift_grole τ /\ *)
+    (*              match ℓ with *)
+    (*              | Take_step _ τ' | Silent_step τ' => τ = τ' *)
+    (*              | Config_step => False *)
+    (*              end *)
+    (*   | None => match ℓ with *)
+    (*            | Config_step => True *)
+    (*            | _ => False *)
+    (*            end *)
+    (*   end.  *)
+    
+    Definition out_LMF_labels_match (oζ : option Lo) (oℓ: option G) :=
+      match oζ, oℓ with
+      | Some ζ, Some ℓ => lift_grole ℓ = ζ
+      | None, None => True
+      | _, _ => False
+      end. 
+    
+    (* TODO: rename *)
+    Definition lm_exaux_traces_match_gen: out_trace → lmftrace (LM := LM) → Prop :=
+      traces_match 
+        (* labels_match *) out_LMF_labels_match
+        (* live_tids *) state_rel
+        (* locale_step  *) out_step
+        (fmtrans LM_Fair). 
+    
+    From trillium.fairness Require Import trace_lookup.
+    
+    (* TODO: move *)
+    Lemma pred_at_impl {St L : Type} (P Q: St -> option L -> Prop)
+      (IMPL: forall s ol, P s ol -> Q s ol):
+      forall tr i, pred_at tr i P -> pred_at tr i Q.
+    Proof.
+      rewrite /pred_at. intros. 
+      destruct after; intuition; destruct t.
+      all: by apply IMPL.
+    Qed.
+    
+    Let lbl_match (ℓ: Lo) oℓ' := oℓ' = Some ℓ. 
+    
+    Theorem fairness_preserved (extr: out_trace) (auxtr: lmftrace (LM := LM)):
+      infinite_trace extr ->
+      lm_exaux_traces_match_gen extr auxtr ->
+      (forall ζ, fair_by locale_prop lbl_match ζ extr) -> (forall τ, fair_by_group τ auxtr).
+    Proof.
+      intros INF MATCH FAIR_OUT.
+      intros. do 2 red. intros n ASG.
+      pose proof ASG as (δ & NTH & [ρ MAP])%pred_at_trace_lookup.
       
+      edestruct @traces_match_state_lookup_2 as (c & ENTH & RELn); eauto.
+      
+      red in FAIR_OUT. edestruct FAIR_OUT as [m STEP].
+      { eapply pred_at_trace_lookup; eauto. }
+      apply pred_at_or in STEP.
+      
+      apply pred_at_or in STEP. 
+      apply pred_at_trace_lookup in STEP as (c' & ENTH' & STEP).
+      edestruct @traces_match_state_lookup_1 as (δ' & NTH' & RELn'); eauto. 
+      exists m. apply pred_at_trace_lookup. eexists. split; eauto.
+      red. destruct STEP as [EMP | STEP]. 
+      - left. intros [??]. apply EMP. eapply match_locale_prop_states; eauto.  
+      - right.
+        destruct STEP as (?&?&LBLM). 
+        edestruct @traces_match_label_lookup_1 as (ℓ & NTH'l & LBL); eauto.
+        eexists. split; eauto. red in LBL.
+        red in LBLM. subst.
+        destruct ℓ; try done.
+        apply INJlg in LBL. congruence.
+    Qed.      
+    
   End Preservation.
 
 End fairness_preserved.
 
 
 (* TODO: move? *)
-Lemma traces_match_LM_preserves_validity `{LM: LiveModel G M LSI}
+Lemma traces_match_LM_preserves_validity `{LM: LiveModel G M LSI} {LF: LMFairPre LM}
   `{C: Type} {L: Type}
-  (otr: trace C L) (auxtr : auxtrace (LM := LM))
+  (otr: trace C L) (auxtr : lmftrace (LM := LM))
   state_rel lbl_rel outer_step :
-  traces_match lbl_rel state_rel outer_step LM.(lm_ls_trans) otr auxtr ->
-  auxtrace_valid auxtr (LM := LM).
+  traces_match lbl_rel state_rel outer_step ((fmtrans LM_Fair)) otr auxtr ->
+  mtrace_valid auxtr.
 Proof.
-  revert otr auxtr. cofix CH. intros otr auxtr Hmatch.
-  inversion Hmatch; first by constructor.
-  constructor =>//. by eapply CH.
+  revert otr auxtr. pcofix CH. intros otr auxtr Hmatch.
+  pfold. 
+  inversion Hmatch; [by econstructor| ].
+  constructor =>//.
+  specialize (CH _ _ H3).
+  eauto.   
 Qed.
 
 Section lang_fairness_preserved.
   Context `{LM: LiveModel (locale Λ) M LSI}.
-  Context `{EqDecision (locale Λ)}.
+  (* Context `{EqDecision (locale Λ)}. *)
+  Context {LF: LMFairPre LM}. 
 
   Definition lm_exaux_traces_match :=
     lm_exaux_traces_match_gen
@@ -468,10 +402,10 @@ Section lang_fairness_preserved.
     have Hv: Some v ≠ None by []. by specialize (Hneqloc Hv ρ).
   Qed.
 
-  Theorem ex_fairness_preserved (extr: extrace Λ) (auxtr: auxtrace (LM := LM)):
+  Theorem ex_fairness_preserved (extr: extrace Λ) (auxtr: lmftrace (LM := LM)):
     infinite_trace extr ->
     lm_exaux_traces_match extr auxtr ->
-    (forall ζ, fair_ex ζ extr) -> (forall ρ, fair_aux ρ auxtr (LM := LM)).
+    (forall ζ, fair_ex ζ extr) -> (∀ ρ : fmrole M, fair_by_next_TS ρ auxtr).
   Proof.
     intros. eapply group_fairness_implies_role_fairness; eauto. 
     { eapply traces_match_infinite_trace; eauto. }
@@ -486,7 +420,8 @@ End lang_fairness_preserved.
 
 Section model_fairness_preserved.
   Context `{LM: LiveModel G M LSI}.
-  Context `{EqDecision G}.
+  (* Context `{EqDecision G}. *)
+  Context {LF: LMFairPre LM}. 
 
   Context `{Mout: FairModel}. 
 
@@ -505,10 +440,10 @@ Section model_fairness_preserved.
       lift_grole
       state_rel. 
   
-  Theorem model_fairness_preserved (mtr: mtrace Mout) (auxtr: auxtrace (LM := LM)):
+  Theorem model_fairness_preserved (mtr: mtrace Mout) (auxtr: lmftrace (LM := LM)):
     infinite_trace mtr ->
     lm_model_traces_match mtr auxtr ->
-    (∀ ρ, fair_model_trace ρ mtr) -> (forall ρ, fair_aux ρ auxtr (LM := LM)).
+    (∀ ρ, fair_model_trace ρ mtr) -> (∀ ρ : fmrole M, fair_by_next_TS ρ auxtr).
   Proof.
     intros. eapply group_fairness_implies_role_fairness; eauto. 
     { eapply traces_match_infinite_trace; eauto. }
